library/Tracing.thy
@@ -1,0 +1,75 @@
+theory Tracing
+  imports Main Refine_Imperative_HOL.Sepref
+begin
+
+datatype message = ExploredState
+
+definition write_msg :: "message \<Rightarrow> unit" where
+  "write_msg m = ()"
+
+code_printing code_module "Tracing" \<rightharpoonup> (SML)
+\<open>
+structure Tracing : sig
+  val count_up : unit -> unit
+  val get_count : unit -> int
+end = struct
+  val counter = Unsynchronized.ref 0;
+  fun count_up () = (counter := !counter + 1);
+  fun get_count () = !counter;
+end
+\<close>
+
+code_reserved SML Tracing
+
+code_printing
+  constant write_msg \<rightharpoonup> (SML) "(fn x => Tracing.count'_up ()) _"
+
+definition trace where
+  "trace m x = (let a = write_msg m in x)"
+
+lemma trace_alt_def[simp]:
+  "trace m x = (\<lambda> _. x) (write_msg x)"
+  unfolding trace_def by simp
+
+definition
+  "test m = trace ExploredState ((3 :: int) + 1)"
+
+definition "TRACE m = RETURN (trace m ())"
+
+lemma TRACE_bind[simp]:
+  "do {TRACE m; c} = c"
+  unfolding TRACE_def by simp
+
+lemma [sepref_import_param]:
+  "(trace, trace) \<in> \<langle>Id,\<langle>Id,Id\<rangle>fun_rel\<rangle>fun_rel"
+  by simp
+
+sepref_definition TRACE_impl is
+  "TRACE" :: "id_assn\<^sup>k \<rightarrow>\<^sub>a unit_assn"
+  unfolding TRACE_def by sepref
+
+lemmas [sepref_fr_rules] = TRACE_impl.refine
+
+
+text \<open>Somehow Sepref does not want to pick up TRACE as it is, so we use the following workaround:\<close>
+
+definition "TRACE' = TRACE ExploredState"
+
+definition "trace' = trace ExploredState"
+
+lemma TRACE'_alt_def:
+  "TRACE' = RETURN (trace' ())"
+  unfolding TRACE_def TRACE'_def trace'_def ..
+
+lemma [sepref_import_param]:
+  "(trace', trace') \<in> \<langle>Id,Id\<rangle>fun_rel"
+  by simp
+
+sepref_definition TRACE'_impl is
+  "uncurry0 TRACE'" :: "unit_assn\<^sup>k \<rightarrow>\<^sub>a unit_assn"
+  unfolding TRACE'_alt_def
+  by sepref
+
+lemmas [sepref_fr_rules] = TRACE'_impl.refine
+
+end
